src/goose_lang/recovery_adequacy.v
@@ -12,14 +12,14 @@ Set Default Proof Using "Type".
 Theorem heap_recv_adequacy `{ffi_sem: ext_semantics} `{!ffi_interp ffi} {Hffi_adequacy:ffi_interp_adequacy} Σ `{hPre: !heapPreG Σ} s k e r σ φ φr φinv Φinv (HINIT: ffi_initP σ.(world)) :
   (∀ `{Hheap : !heapG Σ},
      ⊢ (ffi_start (heapG_ffiG) σ.(world) -∗ trace_frag σ.(trace) -∗ oracle_frag σ.(oracle) ={⊤}=∗
-       □ (∀ n σ κ, state_interp σ κ n -∗ |NC={⊤, ∅}=> ⌜ φinv σ ⌝) ∗
+       □ (∀ n ns σ κ, state_interp σ ns κ n -∗ |NC={⊤, ∅}=> ⌜ φinv σ ⌝) ∗
        □ (∀ hG (Hpf: @heapG_invG _ _ _ _ Hheap = @heapG_invG _ _ _ _ hG),
-                     Φinv hG -∗ □ ∀ σ κ n, state_interp σ κ n -∗ |NC={⊤, ∅}=> ⌜ φinv σ ⌝) ∗
+                     Φinv hG -∗ □ ∀ σ ns κ n, state_interp σ ns κ n -∗ |NC={⊤, ∅}=> ⌜ φinv σ ⌝) ∗
         wpr s k ⊤ e r (λ v, ⌜φ v⌝) Φinv (λ _ v, ⌜φr v⌝))) →
   recv_adequate (CS := goose_crash_lang) s e r σ (λ v _, φ v) (λ v _, φr v) φinv.
 Proof.
   intros Hwp.
-  eapply (wp_recv_adequacy_inv _ _ _ heap_namesO _ _ _ _ _ _ _ _ (λ Hinv Hc names, Φinv (heap_update_pre _ _ Hinv Hc (@pbundleT _ _ names)))).
+  eapply (wp_recv_adequacy_inv _ _ _ heap_namesO _ _ _ _ _ _ _ _ (λ Hinv Hc names, Φinv (heap_update_pre _ _ Hinv Hc (@pbundleT _ _ names))) (λ n, n)).
   iIntros (???) "".
   iMod (na_heap_name_init tls σ.(heap)) as (name_na_heap) "Hh".
   iMod (proph_map_name_init _ κs σ.(used_proph_id)) as (name_proph_map) "Hp".
@@ -32,32 +32,40 @@ Proof.
   set (hG := heap_update_pre _ hPre Hinv Hc hnames).
   iExists ({| pbundleT := hnames |}).
   iExists
-    (λ t σ κs, let _ := heap_update Σ hG Hinv Hc (@pbundleT _ _ t) in
-               state_interp σ κs O)%I,
+    (λ t σ ns κs nt, let _ := heap_update Σ hG Hinv Hc (@pbundleT _ _ t) in
+               state_interp σ ns κs nt)%I,
     (λ t _, True%I).
-  iExists (λ _ _, eq_refl).
+  iExists _. (* (λ Hc t, λ (σ0 : state) (_ : nat) (κs0 : list observation) (_ : nat),
+                                              lifting.heapG_irisG_obligation_1 Σ
+                                                (heap_update Σ (heap_update_pre Σ hPre Hinv Hc hnames) Hinv Hc
+                                                   pbundleT) σ0 κs0). *)
+  iExists _.
+  iExists _.
   iMod (Hwp hG with "[$] [$] [$]") as "(#H1&#H2&Hwp)".
   iModIntro.
   iSplitR.
-  { iModIntro. iIntros (??) "H". rewrite heap_update_pre_update.
+  { iModIntro. iIntros (????) "H". rewrite heap_update_pre_update.
     by iApply "H1".
   }
   iSplitR.
   {
     iModIntro. iIntros (Hc' names') "H". rewrite ?heap_update_pre_update.
     iDestruct ("H2" $! _ _ with "H") as "#H3".
-    iModIntro. iIntros (??) "H". iSpecialize ("H3" with "H").
+    iModIntro. iIntros (????) "H". iSpecialize ("H3" with "H").
     eauto.
   }
   iFrame. rewrite /hG//=.
   rewrite ffi_update_pre_update //=. iFrame.
   rewrite /wpr. rewrite /hG//=.
   rewrite heap_update_pre_get.
+  rewrite //=.
   iApply (recovery_weakestpre.wpr_strong_mono with "Hwp").
   repeat iSplit; [| iModIntro; iSplit]; eauto.
   iIntros. rewrite heap_update_pre_update. eauto.
   Unshelve.
   - eauto.
+  - (* TODO: where is this coming from? *)
+    exact O.
   - (* TODO: where is this coming from? *)
     exact O.
 Qed.
