src/program_logic/staged_wpc.v
@@ -82,11 +82,11 @@ Qed.
 Definition wpc_no_fupd s k mj E1 e1 Φ Φc :=
   ((match to_val e1 with
    | Some v => ∀ q, NC q -∗ |={E1}=> Φ v ∗ NC q
-   | None => ∀ q σ1 κ κs n,
-      state_interp σ1 (κ ++ κs) n -∗ NC q -∗ |={E1,∅}=>
+   | None => ∀ q σ1 ns κ κs n,
+      state_interp σ1 ns (κ ++ κs) n -∗ NC q -∗ |={E1,∅}=> |={∅}▷=>^(S $ num_laters_per_step ns)
         (⌜if s is NotStuck then reducible e1 σ1 else True⌝ ∗
-        ∀ e2 σ2 efs, ⌜prim_step e1 σ1 κ e2 σ2 efs⌝ -∗ |={∅,∅}=> ▷ |={∅,E1}=>
-          (state_interp σ2 κs (length efs + n) ∗
+        ∀ e2 σ2 efs, ⌜prim_step e1 σ1 κ e2 σ2 efs⌝ -∗ |={∅,E1}=>
+          (state_interp σ2 (S ns) κs (length efs + n) ∗
           wpc0 s k mj E1 e2 Φ Φc ∗
           ([∗ list] i ↦ ef ∈ efs, wpc0 s k mj ⊤ ef fork_post True) ∗
           NC q))
@@ -195,7 +195,7 @@ Proof.
     iMod (fupd_split_level_le with "H"); first (naive_solver lia).
     by iDestruct ("HΦcwand" with "[$]") as ">$".
   }
-  iIntros (?????) "Hinterp HNC".
+  iIntros (??????) "Hinterp HNC".
   iDestruct (NC_split with "HNC") as "(HNC1&HNC2)".
   iPoseProof (staged_inv_later_open' E1 _ _ _ _ _ _ _ _ _ (NC (q0/2)) True%I
                                        (wpc_no_fupd NotStuck k'' _ E1 e
@@ -213,13 +213,14 @@ Proof.
   }
   iDestruct "Hwp" as "(H&_)".
   rewrite Hval.
-  iMod ("H" with "[$] [$]") as "(%&H)".
+  iMod ("H" with "[$] [$]") as "H".
+  iModIntro.
+  simpl. iMod "H". iModIntro. iNext. iMod "H". iModIntro.
+  iApply (step_fupdN_wand with "H"). iIntros "(%&H)".
   iSplitL "".
   { by destruct s; auto. }
-  iModIntro.
   iIntros. iMod ("H" with "[//]") as "H".
-  iModIntro. iNext.
-  iMod "H" as "(Hσ&H&Hefs&HNC)".
+  iDestruct "H" as "(Hσ&H&Hefs&HNC)".
   iEval (rewrite wpc0_unfold /wpc_pre) in "H". iMod "H".
   rewrite own_discrete_fupd_eq /own_discrete_fupd_def.
   iDestruct (own_discrete_elim_conj with "H") as (Q_keep Q_inv) "(HQ_keep&HQ_inv&#Hwand1&#Hwand2)".
@@ -348,7 +349,7 @@ Proof.
     iDestruct "Hwp" as "(Hwp&_)". iModIntro. iIntros. by iModIntro.
   }
   rewrite Hval.
-  iIntros (?????) "Hstate HNC".
+  iIntros (??????) "Hstate HNC".
   iDestruct (NC_split with "HNC") as "(Hnc1&Hnc2)".
 
   iPoseProof (staged_inv_open_modify_ae E1 _ _ _ _ _ _ _ _ _ _ (NC (q/2)) True%I (▷Q)%I
@@ -367,13 +368,14 @@ Proof.
   rewrite Hval.
   iSpecialize ("Hwp" with "[$]").
   iMod ("Hwp" $! (S j')) as "(H&_)".
-  iMod ("H" with "[$] [$]") as "(%&H)".
+  iMod ("H" with "[$] [$]") as "H".
+  simpl. iMod "H". iModIntro. iModIntro. iNext. iMod "H". iModIntro.
+  iApply (step_fupdN_wand with "H"). iIntros "(%&H)".
   iSplitL "".
   { destruct s; eauto. }
-  iModIntro. iIntros.
+  iIntros.
   iMod ("H" with "[//]") as "H".
-  iModIntro. iNext.
-  iMod "H" as "(Hσ&H&Hefs&HNC)".
+  iDestruct "H" as "(Hσ&H&Hefs&HNC)".
   iEval (rewrite wpc0_unfold /wpc_pre) in "H". iMod "H".
   rewrite own_discrete_fupd_eq /own_discrete_fupd_def.
   iDestruct (own_discrete_elim_conj with "H") as (Q_keep Q_inv) "(HQ_keep&HQ_inv&#Hwand1&#Hwand2)".
